WIP

theories/Dot/examples/typingExamplesUnst.v
@@ -674,3 +674,215 @@ Proof.
     eapply LSel_stp'; tcrush.
     varsub; tcrush.
 Qed.
+
+Definition loopDefV : vl := ν {@ (* self => *)
+  val "loop" = vabs (tapp (tproj (tv x1) "loop") (tv x0))
+  (* λ v, self.loop v. *)
+}.
+Definition loopDefTConcr : ty := μ {@ val "loop" : ⊤ →: ⊥ }.
+Definition loopDefT : ty := val "loop" : ⊤ →: ⊥.
+Example loopDefTyp Γ : Γ u⊢ₜ tv loopDefV : loopDefT.
+Proof.
+  apply (Subs_typed_nocoerce loopDefTConcr).
+  - tcrush; cbv.
+    eapply App_typed; last var. tcrush.
+    varsub. cbv. lThis.
+  - apply Bind1; tcrush.
+Qed.
+
+Definition loopTm := tapp (tproj (tv loopDefV) "loop") (tv (vnat 0)).
+Example loopTyp Γ : Γ u⊢ₜ loopTm : ⊥.
+Proof.
+  pose proof loopDefTyp Γ.
+  apply (App_typed (T1 := ⊤)); tcrush.
+  apply (Subs_typed_nocoerce 𝐍); tcrush.
+Qed.
+
+Section listLib.
+Context Γ.
+(* bool : boolImplT *)
+Let Γ' := boolImplT :: Γ.
+
+Definition trueTm := tskip (tproj (tv x0) "true").
+Definition falseTm := tskip (tproj (tv x0) "false").
+
+Lemma trueTyp Γ'' : Γ'' ++ Γ' u⊢ₜ trueTm.|[ren (+length Γ'')] : p0.|[ren (+length Γ'')] @; "Boolean".
+Proof.
+  have ?: length Γ'' < length (Γ'' ++ Γ') by rewrite app_length /Γ'/=; lia.
+  rewrite /trueTm /= -(iterate_S tskip 0).
+  apply (Subs_typed (T1 := ▶ pv (ids (length Γ'')) @; "Boolean"));
+    rewrite plusnO; tcrush.
+  eapply Subs_typed_nocoerce.
+  - eapply TMuE_typed'; first eapply Var_typed'; by [rewrite lookup_app_r ?Nat.sub_diag|].
+  - repeat lNext.
+Qed.
+
+Lemma falseTyp Γ'' : Γ'' ++ Γ' u⊢ₜ falseTm.|[ren (+length Γ'')] : p0.|[ren (+length Γ'')] @; "Boolean".
+Proof.
+  have ?: length Γ'' < length (Γ'' ++ Γ') by rewrite app_length /Γ'/=; lia.
+  rewrite /falseTm /= -(iterate_S tskip 0).
+  apply (Subs_typed (T1 := ▶ pv (ids (length Γ'')) @; "Boolean"));
+    rewrite plusnO; tcrush.
+  eapply Subs_typed_nocoerce.
+  - eapply TMuE_typed'; first eapply Var_typed'; by [rewrite lookup_app_r ?Nat.sub_diag|].
+  -
+    (* Optional tactic, just for seeing what happens: *)
+    lNext; rewrite -(decomp_s _ (ids _ .: ren _)) /=.
+    (* Needed: *)
+    repeat lNext.
+Qed.
+(* Definition consTResConcr U : ty := listTBodyGen U U. *)
+(* Definition consTResConcr U : ty := listTBodyGen U U. *)
+(* Eval cbv in listTBodyGen ⊥ (p0 @; "T").
+Eval cbv in (listTBodyGen ⊥ (p1 @; "T")).|[ids 1 .: ids 0 .: ids]. *)
+
+Definition listTBodyGen2 L U := μ {@ (* self => *)
+  type "A" >: shift L <: shift U;
+  val "isEmpty" : ⊤ →: p3 @; "Boolean"; (* bool.Boolean *)
+  val "head" : ⊤ →: p0 @; "A"; (* self.A *)
+  val "tail" : ⊤ →: TAnd (p2 @; "List") (type "A" >: ⊥ <: p0 @; "A" )
+}.
+Definition consTResConcr2 U : ty := listTBodyGen2 U U.
+
+Definition consTConcr2 sci : ty :=
+  TAll (tparam "T")
+    (p0 @; "T" →:
+    TAnd (shift sci @; "List") (type "A" >: ⊥ <: p0 @; "T") →:
+    (consTResConcr2 (p0 @; "T"))).
+    (* shift (consTResConcr2 (p1 @; "T")).|[ids 1 .: ids 0 .: ids]). *)
+
+Eval cbv in consTConcr2 p0.
+
+Definition listTBodyGen L U := μ {@ (* self => *)
+  type "A" >: shift L <: shift U;
+  val "isEmpty" : ⊤ →: p1 @; "Boolean"; (* bool.Boolean *)
+  val "head" : ⊤ →: p0 @; "A"; (* self.A *)
+  val "tail" : ⊤ →: TAnd (p0 @; "List") (type "A" >: ⊥ <: p0 @; "A" )
+}.
+
+Definition listTBody := Eval hnf in listTBodyGen ⊥ ⊤.
+Print listTBody.
+
+Definition nilTConcr : ty := listTBodyGen ⊥ ⊥.
+Definition nilT := TAnd listTBody (typeEq "A" ⊥).
+(* XXX reorder *)
+Definition listTConcrBody : ty := {@ (* sci => *)
+  typeEq "List" $ shift listTBody; (* [shift] is for [sci] *)
+  val "nil" : shift nilT;
+  val "cons" : consTConcr2 p0
+}.
+Definition listTConcr : ty := μ listTConcrBody.
+
+Definition nilV : vl := ν {@ (* self => *)
+  type "A" = ⊥;
+  val "isEmpty" = vabs (* d => *) (trueTm.|[ren (+2)]); (* for self and d *)
+  val "head" = vabs loopTm;
+  val "tail" = vabs loopTm
+}.
+
+Example nilTyp : (▶ listTConcrBody)%ty :: Γ' u⊢ₜ shift (tv nilV) : shift nilT.
+Proof.
+  apply (Subs_typed_nocoerce (shift nilTConcr)).
+  - evar (T : ty).
+    have := trueTyp [⊤; T; ▶ listTConcrBody]%ty.
+    have := loopTyp (⊤ :: T :: ▶ listTConcrBody :: Γ')%ty.
+    rewrite {}/T/= => Ht Hl. cbv.
+    (* tcrush. *)
+    tcrush; apply (Subs_typed_nocoerce ⊥); tcrush.
+  - tcrush.
+    lThis.
+    apply Bind1; tcrush.
+Qed.
+(* ∀(x: {A})∀(hd: x.A)∀(tl: sci.List∧{A <: x.A})sci.List∧{A <: x.A} *)
+
+(* Definition consTConcr sci : ty :=
+  TAll (tparam "T")
+    (p0 @; "T" →:
+    TAnd (shift sci @; "List") (type "A" >: ⊥ <: p0 @; "T") →:
+    (consTResConcr (p1 @; "T")).|[ids 1 .: ids 0 .: ids]). *)
+(* .|[upn 1 (ren (+1))] *)
+
+Definition consT sci : ty :=
+  TAll (tparam "T")
+    (p0 @; "T" →:
+    (TAnd (shift sci @; "List") (type "A" >: ⊥ <: p0 @; "T")) →:
+    TAnd (shift sci @; "List") (type "A" >: ⊥ <: p0 @; "T")).
+(*
+  λ(x: {A})λ(hd: x.A)λ(tl: sci.List∧{A <: x.A}) let result = ν(self) {
+  A = x.A; isEmpty = bool.false; head = hd; tail = tl } in result *)
+Definition consV : vl :=
+  vabs (* x => *) $ vabs' (* hd => *) $ vabs' (* tl => *) $ tv $ ν {@ (* self => *)
+    type "A" = p3 @; "T";
+    val "isEmpty" = vabs (* d => *) falseTm.|[ren (+5)];
+    val "head" = vabs (* d => *) (tv x3);
+    val "tail" = vabs (* d => *) (tv x2)
+  }.
+
+Example consTyp :
+  (▶ listTConcrBody)%ty :: Γ' u⊢ₜ shift (tv consV) : consTConcr2 p0.
+Proof.
+  cbv.
+(* Eval cbv in (consTResConcr (p1 @; "T")).|[ids 1 .: ids 0 .: ids]. *)
+  epose proof falseTyp [_; _; _; _; _; _] as Ht; cbn in Ht.
+  (* evar (T : ty).
+  have HT := falseTyp [⊤%ty; T; ▶ listTConcrBody]%ty. *)
+  tcrush; clear Ht; first by varsub; eapply (LSel_stp' _ (p4 @; "T")); tcrush; varsub; lThis.
+  cbv; hideCtx. varsub. cbn. tcrush. lNext.
+  eapply LSel_stp'; tcrush. varsub. lThis.
+Qed.
+
+Lemma consTSub : listTConcrBody :: Γ' u⊢ₜ consTConcr2 p0, 0 <: consT p0, 0.
+Proof.
+  cbv.
+  tcrush; rewrite !iterate_S !iterate_0; hideCtx.
+  2: {
+    apply Bind1; stcrush. lThis.
+  }
+  eapply LSel_stp'; tcrush. varsub. tcrush. lThis.
+  by lThis.
+  repeat lNext.
+  repeat lNext.
+  cbn. simplSubst.
+  rewrite !iterate_0.
+  do 3 lNext. cbn. simplSubst.
+  lThis. rewrite !iterate_S !iterate_0.
+  tcrush.
+  (* rewrite /consT /consTConcr /consTResConcr.
+  tcrush. apply Bind1; tcrush.
+  cbv; hideCtx.
+  eapply LSel_stp'; stcrush. *)
+  (* varsub. *)
+Admitted.
+
+
+Notation shiftV v := v.[ren (+1)].
+Definition listV : vl := ν {@ (* sci => *)
+  type "List" = shift listTBody; (* [shift] is for [sci] *)
+  val "nil" = shiftV nilV;
+  val "cons" = shiftV consV
+}.
+
+Definition listT : ty := μ {@ (* sci => *)
+  type "List" >: ⊥ <: shift listTBody; (* [shift] is for [sci] *)
+  val "nil" : shift nilT;
+  val "cons" : consT p0
+}.
+
+Example listTypConcr : Γ' u⊢ₜ tv listV : listTConcr.
+Admitted.
+
+Example listTyp : Γ' u⊢ₜ tv listV : listT.
+Proof.
+  have := listTypConcr.
+  have := consTSub.
+  have := consTyp.
+  have := nilTyp => *.
+  (* evar (U : ty); have := nilTyp U; rewrite {}/U => Ht. *)
+
+  apply (Subs_typed_nocoerce listTConcr); tcrush.
+  lThis.
+  lNext.
+  do 2 lNext; lThis.
+Qed.
+
+End listLib.
